Modularisation of hmac proof, part 2: isolate sha-dependences

sha/HMAC_common_defs.v
@@ -1,28 +1,73 @@
 Require Import Integers.
 Require Import Recdef.
-Require Import List. Import ListNotations.
-Require Import Arith.
-Require Import Coqlib.
-Require Import pure_lemmas.
-Require Import SHA256.
+Require Import Bvector. 
+Require Import List. Import ListNotations. 
+Require Import Arith. 
+Require Import Coqlib. 
+Require Import general_lemmas. 
 Require Import hmac_pure_lemmas.
-Require Import sha_padding_lemmas.
+Require Import XorCorrespondence.
 Require Import ByteBitRelations.
-Require Import HMAC_functional_prog.
-Require Import hmac_common_lemmas.
-
-Definition Blist := list bool.
 
 Definition concat {A : Type} (l : list (list A)) : list A :=
   flat_map id l.
+
+Lemma concat_length {A}: forall L (l:list A), In l L -> (length (concat L) >= length l)%nat.
+Proof.  unfold concat. induction L; simpl; intros. contradiction.
+  rewrite app_length. 
+  destruct H; subst. unfold id. omega.
+  specialize (IHL _ H). omega.
+Qed.
+
+Lemma concat_InBlocks b: forall l (F: Forall (fun x : list bool => length x = b) l),
+      InBlocks b (concat l).
+induction l; simpl; intros. constructor.
+econstructor. 2: reflexivity.
+ apply Forall_inv in F; trivial.
+ apply IHl. apply Forall_tl in F; trivial.
+Qed. 
+
+Lemma concat_app {A} (l1 l2:list A): l1 ++ l2 = l1 ++ concat (l2 :: nil).
+Proof. 
+  unfold concat. simpl.
+  rewrite -> app_nil_r. reflexivity.
+Qed.
 
 (* Replacing splitVector *)
 Definition splitList {A : Type} (n : nat) (l : list A) : (list A * list A) :=
   (firstn n l, skipn n l).
 
+Lemma split_append_id : forall {A : Type} (len : nat) (l1 l2 : list A),
+                               length l1 = len -> length l2 = len ->
+                               splitList len (l1 ++ l2) = (l1, l2).
+Proof.
+  induction len; intros l1 l2 len1 len2.
+  - apply list_nil in len1; apply list_nil in len2. 
+    subst. reflexivity.
+  - unfold splitList.
+    rewrite -> firstn_exact. rewrite -> skipn_exact.
+    * reflexivity. * assumption. * assumption.
+Qed.
+
 (* Replacing BVxor *)
 Definition BLxor (xs : Blist) (ys : Blist) :=
   map (fun p => xorb (fst p) (snd p)) (combine xs ys).
+
+Lemma BLxor_length: forall n l1 l2
+      (len1: length l1 = n) (len2: length l2 = n), length (BLxor l1 l2) = n.
+Proof.
+  induction n as [ | n']; intros.
+  - apply list_nil in len1. apply list_nil in len2.
+    subst. reflexivity.
+  - destruct l1; destruct l2; inversion len1; inversion len2.
+    simpl.
+    rewrite -> map_length.
+    rewrite -> combine_length.
+    rewrite H0. rewrite H1. simpl.
+    f_equal.
+    apply min_l.
+    omega.
+Qed.
 
 Theorem xor_eq : forall (n : nat) (v1 v2 : Bvector.Bvector n),
                    BLxor (Vector.to_list v1) (Vector.to_list v2) = 
@@ -35,375 +80,69 @@ Proof.
    rewrite VectorToList_combine. reflexivity.
 Qed.
  
-Function hash_blocks_bits (hash_block_bit : Blist -> Blist -> Blist) (r: Blist)
+Lemma inner_general_mapByte : forall (ip : Blist) (IP_list : list byte) (k : Blist) (K : list byte),
+                            bytes_bits_lists ip (map Byte.unsigned IP_list) ->
+                            bytes_bits_lists k (map Byte.unsigned K) ->
+     bytes_bits_lists (BLxor k ip)
+                      (map Byte.unsigned
+                           (map (fun p0 : byte * byte => Byte.xor (fst p0) (snd p0))
+                                (combine K IP_list))).
+Proof.
+  intros ip IP_list k K ip_eq k_eq.
+  unfold BLxor. simpl.
+  remember (map Byte.unsigned IP_list). remember (map Byte.unsigned K) as KL.
+  generalize dependent K. generalize dependent IP_list. generalize dependent ip. generalize dependent l.
+  induction k_eq.
+  - simpl; intros. destruct K; simpl in *. constructor. discriminate.
+  - intros l ip ip_eq.
+    induction ip_eq; simpl; intros.
+    + destruct IP_list; simpl in *. 2: discriminate.
+      destruct K; simpl in *. discriminate. constructor.
+    + destruct IP_list. discriminate. simpl in Heql. inversion Heql; clear Heql. subst byte0 bytes0.
+      destruct K; simpl in HeqKL. discriminate. inversion HeqKL; clear HeqKL; subst.
+      simpl.
+      constructor.
+      * eapply IHk_eq; try reflexivity.
+        apply ip_eq.
+      * unfold Byte.xor. rewrite Byte.unsigned_repr.
+        apply xor_correspondence. apply H. apply H0.
+        destruct (@isbyteZ_xor (Byte.unsigned i0) (Byte.unsigned i)).
+        apply isByte_ByteUnsigned.
+        apply isByte_ByteUnsigned. 
+        assert (BMU: Byte.max_unsigned = 255). reflexivity. omega.
+Qed.
+
+Function hash_blocks_bits (b:nat) (B:(0<b)%nat) (hash_block_bit : Blist -> Blist -> Blist) (r: Blist)
          (msg: Blist) {measure length msg} : Blist :=
   match msg with
   | nil => r
-  | _ => hash_blocks_bits hash_block_bit (hash_block_bit r (firstn 512 msg)) (skipn 512 msg)
+  | _ => hash_blocks_bits b B hash_block_bit (hash_block_bit r (firstn b msg)) (skipn b msg)
   end.
 Proof. intros.
- destruct (lt_dec (length msg) 512). 
+ destruct (lt_dec (length msg) b). 
  rewrite skipn_short. simpl; omega. rewrite <- teq; omega.
- rewrite skipn_length. simpl; omega. rewrite <- teq; omega.
+ rewrite skipn_length; rewrite <- teq; omega. 
 Defined.
-
-
-(* TODO use neater definition with conversion functions *)
-(* TODO split out of HMAC_spec_pad *)
-
-Definition c := (32 * 8)%nat.
-Definition p := (32 * 8)%nat.
-Definition b := (c + p)%nat.
-Definition BlockSize := 64.
-Definition BlockSize_Bits := BlockSize * 8.
-
-Definition intsToBits (l : list int) : list bool :=
-  bytesToBits (SHA256.intlist_to_Zlist l).
-
-Definition bitsToInts (l : Blist) : list int :=
-  SHA256.Zlist_to_intlist (bitsToBytes l).
-
-Definition sha_iv : Blist :=
-  intsToBits SHA256.init_registers.
-
-Definition sha_h (regs : Blist) (block : Blist) : Blist :=
-  intsToBits (SHA256.hash_block (bitsToInts regs) (bitsToInts block)).
-
-Definition sha_splitandpad (msg : Blist) : Blist :=
-  bytesToBits (sha_padding_lemmas.pad (bitsToBytes msg)).
-
-(* artifact of app_fpad definition *)
-Definition fpad_inner (msg : list Z) : list Z :=
-  (let n := BlockSize + Zlength msg in
-  [128%Z]
-    ++ list_repeat (Z.to_nat (-(n + 9) mod 64)) 0
-    ++ intlist_to_Zlist ([Int.repr (n * 8 / Int.modulus); Int.repr (n * 8)]))%list.
-
-Definition fpad (msg : Blist) : Blist :=
-  bytesToBits (fpad_inner (bitsToBytes msg)).
-
-(* --------------- *)
-
-Lemma BLxor_length : forall (l1 l2 : Blist) (n : nat),
-                       length l1 = n ->
-                       length l2 = n ->
-                       length (BLxor l1 l2) = n.
-Proof.
-  intros l1 l2 n len1 len2.
-  revert l1 l2 len1 len2.
-  induction n as [ | n'].
-  - intros. apply list_nil in len1. apply list_nil in len2.
-    subst. reflexivity.
-  - intros l1 l2 len1 len2.
-    destruct l1; destruct l2; inversion len1; inversion len2.
-    simpl.
-    rewrite -> map_length.
-    rewrite -> combine_length.
-    rewrite H0. rewrite H1. simpl.
-    f_equal.
-    apply min_l.
-    omega.
-Qed.
-
-Lemma split_append_id : forall {A : Type} (len : nat) (l1 l2 : list A),
-                               length l1 = len -> length l2 = len ->
-                               splitList len (l1 ++ l2) = (l1, l2).
-Proof.
-  induction len; intros l1 l2 len1 len2.
-  -
-    assert (H: forall {A : Type} (l : list A), length l = 0%nat -> l = []).
-      intros. destruct l.
-      reflexivity. inversion H.
-    apply H in len1. apply H in len2.
-    subst. reflexivity.
-  -
-    unfold splitList.
-    rewrite -> firstn_exact. rewrite -> skipn_exact.
-    * reflexivity. * assumption. * assumption.
-Qed.
-
-
-Lemma fold_left_iv_length: forall k (HK: forall iv x, length iv = k -> length (sha_h iv x) = k) l iv x , 
-  length iv = k ->
-  length (fold_left sha_h l (sha_h iv x)) = k.
-Proof. intros k HK l.
-  induction l. simpl. apply HK. 
-  simpl. intros.  rewrite IHl. trivial. apply HK. trivial.
-Qed. 
-
-
-(* modified version of sha_padding_lemmas.pad *)
-Definition pad_inc (msg : list Z) : list Z := 
-  let n := BlockSize + Zlength msg in
-  msg ++ [128%Z] 
-      ++ list_repeat (Z.to_nat (-(n + 9) mod 64)) 0
-      ++ intlist_to_Zlist ([Int.repr (n * 8 / Int.modulus); Int.repr (n * 8)]).
-
-Definition sha_splitandpad_inc (msg : Blist) : Blist :=
-  bytesToBits (pad_inc (bitsToBytes msg)).
-
-Lemma sha_splitandpad_inc_nil: length (sha_splitandpad_inc nil) = 512%nat.
-Proof. reflexivity. Qed.
 
 Lemma add_blocksize_length l n: 0<=n ->
       BinInt.Z.add n (Zcomplements.Zlength l) = Zcomplements.Zlength ((Coqlib.list_repeat (Z.to_nat n) true) ++ l).
 Proof. intros. do 2 rewrite Zlength_correct.
   rewrite app_length, length_list_repeat, Nat2Z.inj_add, Z2Nat.id; trivial.
-Qed. 
-
-Lemma isbyteZ_pad_inc l (B:Forall isbyteZ l): Forall isbyteZ (pad_inc l).
-Proof. unfold pad_inc.
-  apply Forall_app. split. trivial. 
-  apply Forall_app. split. constructor. split; omega. trivial.
-  apply Forall_app. split. apply Forall_list_repeat. split; omega.
-  apply isbyte_intlist_to_Zlist.
 Qed.
 
-Lemma pad_inc_length: forall l, exists k, (0 < k /\ length (pad_inc l) = k*64)%nat.
-Proof. unfold pad_inc.
-  induction l. 
-  simpl. exists (1%nat). omega.
-  destruct IHl as [k [K HK]]. repeat rewrite app_length in *. rewrite length_list_repeat in *.
-  rewrite pure_lemmas.length_intlist_to_Zlist in *.
-  remember (BinInt.Z.to_nat
-        (BinInt.Z.modulo
-           (BinInt.Z.opp
-              (BinInt.Z.add (BinInt.Z.add BlockSize (Zcomplements.Zlength l))
-                 9)) 64)).
-  remember (BinInt.Z.to_nat
-      (BinInt.Z.modulo
-         (BinInt.Z.opp
-            (BinInt.Z.add
-               (BinInt.Z.add BlockSize (Zcomplements.Zlength (a :: l))) 9))
-         64)).
-  simpl. simpl in HK.
-  assert ((BinInt.Z.add
-                   (BinInt.Z.add BlockSize (Zcomplements.Zlength (a :: l))) 9) =
-          BinInt.Z.add 1 (BinInt.Z.add
-                   (BinInt.Z.add BlockSize (Zcomplements.Zlength l)) 9)).
-        rewrite BinInt.Z.add_assoc. f_equal.
-          rewrite BinInt.Z.add_assoc. rewrite (BinInt.Z.add_comm 1). rewrite <- (BinInt.Z.add_assoc _ 1).
-          f_equal. 
-          repeat rewrite Zcomplements.Zlength_correct. 
-          apply (Znat.Nat2Z.inj_add 1 (length l)).
-   rewrite H in Heqn0; clear H. 
-   remember (BinInt.Z.add (BinInt.Z.add BlockSize (Zcomplements.Zlength l)) 9). clear Heqz.
-   subst n n0. rewrite Z.opp_add_distr. rewrite <- (Z.add_comm (-z)). remember (-z) as zz. clear Heqzz.
-   simpl.
-   destruct (zeq (zz mod 64) 0).
-     rewrite e in HK.
-     assert ((zz+-1) mod 64 = 63). clear - e.  apply Zmod_divides in e. 2:omega. 
-        destruct e. subst. rewrite Zplus_mod. rewrite Z.mul_comm. rewrite Z_mod_mult. simpl.
-        rewrite Zmod_mod. apply Zmod_unique with (a:=(-1)). omega. omega.
-     rewrite H. clear H e. simpl in *. exists (S k). omega.
-   assert ((zz + -1) mod 64 = (zz mod 64) - 1 /\ 0 <= (zz mod 64) - 1). 
-     clear -n. rewrite Zplus_mod. assert (0 <= zz mod 64 < 64). apply Z.mod_pos_bound. omega.
-     split. 2: omega.
-     symmetry. eapply Z.mod_unique. left. omega.
-     assert (63 = -1 mod 64). eapply Z.mod_unique. left; omega. instantiate (1:=-1). omega.
-     rewrite <- H0. instantiate (1:=1). omega.
-   destruct H. rewrite H. clear H.   
-   assert (Z.to_nat (zz mod 64 - 1) = minus (Z.to_nat (zz mod 64)) 1).
-     clear - n H0. remember (zz mod 64).  clear Heqz. rewrite Z2Nat.inj_sub. reflexivity. omega. 
-   rewrite H; clear H. rewrite <- NPeano.Nat.add_sub_swap. rewrite minus_Sn_m. simpl. exists k. omega.
-   omega. apply (Z2Nat.inj_le 1). omega. omega. omega.
-Qed. 
-
-Lemma sha_splitandpad_inc_length: forall m, exists k, 
-      (0<k /\ length (sha_splitandpad_inc m) = k * 512)%nat.
-Proof. intros. unfold sha_splitandpad_inc.
-  destruct (pad_inc_length (bitsToBytes m)) as [k [K HK]].
-  rewrite bytesToBits_len, HK. exists k. split. trivial. omega.
-Qed.
-
-
-Lemma sha_splitandpad_inc_InBlocks m : InBlocks 512 (sha_splitandpad_inc m).
-Proof. intros. apply InBlocks_len.
-  destruct (sha_splitandpad_inc_length m) as [k [K HK]].
-  rewrite HK. exists k. trivial.
-Qed.
-
-Lemma sha_iv_length: length sha_iv = 256%nat.
-Proof. reflexivity. Qed.
-
-Lemma hash_blocks_bits_len: forall r l, length r = 256%nat -> 
-      InBlocks 512 l ->
-      length (hash_blocks_bits sha_h r l) = 256%nat.
-Proof. intros r l.
+Lemma hash_blocks_bits_len c b (B:(0<b)%nat) h 
+          (HH: forall x y, length x = c -> length y = b -> length (h x y)  = c)
+          r l: length r = c -> 
+      InBlocks b l ->
+      length (hash_blocks_bits b B h r l) = c.
+Proof. 
   apply hash_blocks_bits_ind.
   intros. trivial.
   intros. destruct _x. contradiction. subst msg; clear y.
   inv H1.
-  apply H; clear H. unfold sha_h, intsToBits.
- rewrite bytesToBits_len, length_intlist_to_Zlist.
-  rewrite length_hash_block. omega.
-  unfold bitsToInts. erewrite length_Zlist_to_intlist. reflexivity.
-    rewrite bitsToBytes_len_gen with (n:=32%nat). reflexivity. apply H0.
-  unfold bitsToInts. erewrite length_Zlist_to_intlist. reflexivity.
-    erewrite bitsToBytes_len_gen with (n:=64%nat). reflexivity.
-    rewrite H3, firstn_exact. apply H2. apply H2.
-    rewrite H3, skipn_exact. assumption. apply H2. 
+  apply H; clear H. rewrite HH. trivial. trivial.
+    rewrite H3, firstn_exact; trivial. 
+    rewrite H3, skipn_exact; trivial.
 Qed.
+ 
 
-Lemma sha_h_length iv blk: length iv = c -> length blk = b ->
-      length (sha_h iv blk) = c.
-Proof. intros.
- unfold sha_h, intsToBits.
-  rewrite bytesToBits_len, pure_lemmas.length_intlist_to_Zlist.
-  rewrite common_lemmas.length_hash_block. reflexivity.
-  unfold bitsToInts. erewrite pure_lemmas.length_Zlist_to_intlist. reflexivity. 
-  erewrite bitsToBytes_len_gen. reflexivity.
-  rewrite H; reflexivity.
-  unfold bitsToInts. erewrite pure_lemmas.length_Zlist_to_intlist. reflexivity. 
-  erewrite bitsToBytes_len_gen. reflexivity.
-  rewrite H0; reflexivity.
-Qed.
-
-(*******Injectivity of pad_inc*************************)
-
-Lemma pad_injective_aux (l1 l2: list Z) k 
-     (K : k * Int.modulus + (BlockSize + Zlength l1) * 8 =
-          (BlockSize + Zlength l2) * 8)
-     (N : k <> 0):
-     - (BlockSize + Zlength l2 + 9) mod 64 = - (BlockSize + Zlength l1 + 9) mod 64.
-Proof. repeat rewrite <- Z.add_assoc. unfold BlockSize.
-         repeat rewrite Z.opp_add_distr. 
-         rewrite (Zplus_mod (-(64))).
-         assert (- (64) mod 64 = 0). reflexivity. rewrite H.
-         rewrite (Zplus_mod (-(64))). rewrite H. simpl.
-         repeat rewrite Zmod_mod.
-         rewrite Zplus_mod. rewrite (Zplus_mod (- Zlength l1)). 
-         assert (Z12: - Zlength l2 mod 64 = - Zlength l1 mod 64).
-         { clear H. repeat rewrite Z.mul_add_distr_r in K.
-           assert (k * Int.modulus + Zlength l1 * 8 = Zlength l2 * 8). omega.
-           clear K.
-           assert (KK: k * (Int.modulus/8) + Zlength l1 = Zlength l2).
-              rewrite <- (Zdiv_unique (k * Int.modulus + Zlength l1 * 8) 8 (Zlength l2) 0).
-              2: rewrite Z.add_0_r; trivial. 2: omega.
-              clear H. remember (Zlength l1) as z; clear Heqz. 
-              remember ((Int.modulus / 8)).
-              assert (Int.modulus = z0 * 8). subst. 
-                rewrite <- max_unsigned_modulus, int_max_unsigned_eq. trivial.
-              rewrite H; clear H Heqz0. rewrite Z.mul_assoc.
-              rewrite (Z_div_plus_full_l (k*z0) 8 (z*8)). 2: omega. 
-              rewrite Z_div_mult_full. trivial. omega.
-           rewrite <- KK; clear H KK.
-           rewrite Z.opp_add_distr.  
-           rewrite Zplus_mod.
-           assert (KM: - (k * (Int.modulus / 8)) mod 64 = 0).
-             apply Zmod_unique with (a:=-k * 8388608). 2: omega. rewrite Zplus_0_r.
-             rewrite <- max_unsigned_modulus, int_max_unsigned_eq. simpl.
-             rewrite Zopp_mult_distr_l, <- Z.mul_assoc. reflexivity.
-           rewrite KM. simpl. apply Z.mod_mod. omega.
-         } 
-         rewrite Z12; trivial.
-Qed. 
-
-Lemma pad_injective_Case5 l1 l2
-  (H0 : (l1 ++ 128 :: nil) ++
-        list_repeat (Z.to_nat (- (BlockSize + Zlength l1 + 9) mod 64)) 0 =
-        (l2 ++ 128 :: nil) ++
-        list_repeat (Z.to_nat (- (BlockSize + Zlength l2 + 9) mod 64)) 0)
-  (H : (BlockSize + Zlength l1) * 8 =
-       ((BlockSize + Zlength l2) * 8) mod Int.modulus)
-  (Nonneg1 : 0 <= (BlockSize + Zlength l1) * 8)
-  (l : (BlockSize + Zlength l1) * 8 < Int.modulus):
-  length l1 = length l2.
-Proof. symmetry in H.
-       destruct (mod_exists _ _ _ H) as [k K].
-       specialize Int.modulus_pos; intros; omega.
-       destruct (zeq k 0). 
-         subst. clear - K. 
-         assert (Zlength l1 = Zlength l2). omega.
-         repeat rewrite Zlength_correct in H.
-         rewrite <- (Nat2Z.id (length l1)).
-         rewrite <- (Nat2Z.id (length l2)).
-         rewrite H. reflexivity.
-       clear H.
-       assert (length ((l1 ++ 128 :: nil) ++
-                list_repeat (Z.to_nat (- (BlockSize + Zlength l1 + 9) mod 64)) 0) 
-             = length ((l2 ++ 128 :: nil) ++
-                list_repeat (Z.to_nat (- (BlockSize + Zlength l2 + 9) mod 64)) 0)).
-       rewrite H0; trivial.
-       clear H0. repeat rewrite app_length in H.
-       repeat rewrite length_list_repeat in H.
-       clear - K n H.
-       rewrite (pad_injective_aux l1 l2 k K n) in H. omega.
-Qed. 
-
-Lemma pad_inc_injective: forall l1 l2, pad_inc l1 = pad_inc l2 -> l1=l2.
-Proof. intros.
-remember (beq_nat (length l1) (length l2)) as d.
-destruct d.
-{ apply beq_nat_eq in Heqd. 
-  unfold pad_inc in H. repeat rewrite Zlength_correct in H.
-  rewrite <- Heqd in H.
-  eapply app_inv_tail. apply H. }
-{ symmetry in Heqd; apply beq_nat_false in Heqd.
-  unfold pad_inc in H.
-  repeat rewrite app_assoc in H.
-  destruct (app_inv_length2 _ _ _ _ H); clear H. reflexivity.
-  apply pure_lemmas.intlist_to_Zlist_inj in H1.
-  apply cons_inv in H1. destruct H1 as [_ Y].
-  apply cons_inv in Y. destruct Y as [Y _].
-  assert (Int.unsigned (Int.repr ((BlockSize + Zlength l1) * 8)) = Int.unsigned (Int.repr ((BlockSize + Zlength l2) * 8))).
-    rewrite Y; trivial.
-  elim Heqd; clear Heqd Y.
-  repeat rewrite Int.unsigned_repr_eq in H.
-  assert (Nonneg1: 0 <= (BlockSize + Zlength l1) * 8).
-    specialize (Zlength_nonneg l1). intros; unfold BlockSize; omega.
-  assert (Nonneg2: 0 <= (BlockSize + Zlength l2) * 8).
-    specialize (Zlength_nonneg l2). intros; unfold BlockSize; omega.
-  remember (zlt ((BlockSize + Zlength l1) * 8) Int.modulus).
-  destruct s; clear Heqs.
-  {  rewrite Zmod_small in H. 2: split; assumption.
-     remember (zlt ((BlockSize + Zlength l2) * 8) Int.modulus).
-     destruct s; clear Heqs.
-     { (*Case 3*)
-       rewrite Zmod_small in H. 2: split; assumption.
-       clear - H. 
-       assert (Zlength l1 = Zlength l2). omega.
-       repeat rewrite Zlength_correct in H0.
-       rewrite <- (Nat2Z.id (length l1)).
-       rewrite <- (Nat2Z.id (length l2)).
-       rewrite H0. reflexivity. }
-     { (*Case 5*) clear g Nonneg2.
-       apply pad_injective_Case5; assumption. } }
-  { clear g Nonneg1.
-    remember (zlt ((BlockSize + Zlength l2) * 8) Int.modulus).
-    destruct s; clear Heqs.
-    { (*Case 5, symmetric version*)
-       rewrite (Zmod_small ((BlockSize + Zlength l2) * 8)) in H. 2: split; assumption.
-       symmetry. symmetry in H. symmetry in H0.
-       apply pad_injective_Case5; assumption. }
-    { clear Nonneg2 g.   
-      remember ((BlockSize + Zlength l1) * 8) as z1. 
-      remember ((BlockSize + Zlength l2) * 8) as z2. 
-  
-      rewrite Zmod_eq in H. 2: apply Int.modulus_pos. remember (z1 / Int.modulus) as k1; clear Heqk1.
-      rewrite Zmod_eq in H. 2: apply Int.modulus_pos. remember (z2 / Int.modulus) as k2; clear Heqk2.
-      destruct (zeq k1 k2).
-      { subst. clear -H.
-        assert (Zlength l1 = Zlength l2). omega.
-        repeat rewrite Zlength_correct in H0.
-        rewrite <- (Nat2Z.id (length l1)).
-        rewrite <- (Nat2Z.id (length l2)).
-        rewrite H0. reflexivity. }
-      { assert (length ((l1 ++ 128 :: nil) ++
-                 list_repeat (Z.to_nat (- (BlockSize + Zlength l1 + 9) mod 64)) 0) 
-              = length ((l2 ++ 128 :: nil) ++
-                 list_repeat (Z.to_nat (- (BlockSize + Zlength l2 + 9) mod 64)) 0)).
-          rewrite H0; trivial.
-        clear H0. repeat rewrite app_length in H1.
-        repeat rewrite length_list_repeat in H1.
-        rewrite (pad_injective_aux l2 l1 (k1-k2)) in H1.
-          omega. 
-          rewrite Z.mul_sub_distr_r; omega.
-          omega. } } } }
-Qed.
-(********************************************************************)  
-
-Lemma block_8 A (l:list A): length l = b -> InBlocks 8 l.
-Proof.
-  intros len. apply InBlocks_len. exists 64%nat. apply len. 
-Qed.
