sha/HMAC256_spec_concat.v
@@ -1,0 +1,60 @@
+Require Import List. Import ListNotations.
+Require Import general_lemmas.
+Require Import ByteBitRelations.
+Require Import HMAC_spec_concat.
+Require Import HMAC_spec_pad.
+
+(*SHA256-specific files*)
+Require Import sha_padding_lemmas. (*for pad.*)
+Require Import ShaInstantiation.
+
+Lemma fpad_eq : forall (l m : Blist),
+                  length l = b ->
+                  InBlocks 8 m ->
+                  sha_splitandpad (l ++ m) = l ++ HMAC_Concat.app_fpad fpad m.
+Proof.
+  intros l m len len_m.
+  unfold HMAC_Concat.app_fpad.
+  unfold sha_splitandpad. unfold fpad.
+  unfold pad. unfold fpad_inner.
+
+  rewrite -> bitsToBytes_app.
+  repeat rewrite -> bytesToBits_app.
+  repeat rewrite -> bits_bytes_bits_id.
+  rewrite <- app_assoc.
+  rewrite -> Zlength_app.
+  repeat f_equal.
+
+  * apply bitsToBytes_len. apply len.
+  * apply bitsToBytes_len. apply len.
+  * apply bitsToBytes_len. apply len.
+  * apply len_m.
+  * apply block_8. apply len.
+  * apply block_8. apply len.
+Qed. 
+
+Theorem HMAC_concat_pad_sap_instantiated
+        h (HH: forall x y, length x = c -> length y = b -> length (h x y)  = c) 
+        iv (IV: length iv = c) (op ip : Blist) (IL: length ip = b) (OL: length op = b)
+        : forall (k m : Blist), length k = b ->
+  HMAC_Pad.HMAC c p B h iv sha_splitandpad op ip k m =
+  HMAC_Concat.HMAC c p B h iv sha_splitandpad_inc fpad op ip k m.
+Proof. intros.
+  apply HMAC_Concat.HMAC_concat_pad; trivial.
+  exists 32%nat. reflexivity.
+  apply splitandpad_eq.
+  apply fpad_eq.
+  apply sha_splitandpad_inc_InBlocks.
+Qed.
+
+Theorem HMAC_concat_pad_explicit : forall (k m : Blist) (op ip : Blist),
+                            length k = b ->
+                            length ip = b ->
+                            length op = b -> 
+  HMAC_Pad.HMAC c p B sha_h sha_iv sha_splitandpad op ip k m =
+  HMAC_Concat.HMAC c p B sha_h sha_iv sha_splitandpad_inc fpad op ip k m.
+Proof.
+  intros k m op ip len_k len_ip len_op.
+  apply HMAC_concat_pad_sap_instantiated; trivial.
+    apply sha_h_length.
+Qed.
