sha/HMAC256_spec_pad.v
@@ -1,0 +1,157 @@
+Set Implicit Arguments.
+Require Import Coqlib.
+Require Import Integers.
+Require Import general_lemmas.
+Require Import ByteBitRelations.
+Require Import HMAC_common_defs.
+Require Import HMAC_spec_pad.
+
+(*The sha-specific imports*)
+Require Import SHA256. 
+Require Import HMAC_functional_prog. 
+Require Import hmac_common_lemmas.
+Require Import sha_padding_lemmas. (*for pad_len_64_nat*)
+Require Import ShaInstantiation.
+
+(*Derived lemmas
+Lemma front_equiv_SHA256 :
+  forall (back : Blist) (BACK : list int) (front : Blist) (FRONT : list int),
+    (length front)%nat = 512%nat ->
+    (length FRONT)%nat = 16%nat ->
+    front ++ back = convert (FRONT ++ BACK) ->
+    front = convert FRONT.
+Proof. intros. eapply front_equiv; try eassumption. omega. Qed. 
+
+Lemma back_equiv_SHA256 :
+  forall (back : Blist) (BACK : list int) (front : Blist) (FRONT : list int),
+    (length front)%nat = 512%nat ->
+    (length FRONT)%nat = 16%nat ->
+    front ++ back = convert (FRONT ++ BACK) ->
+    back = convert BACK.
+Proof. intros. eapply back_equiv; try eassumption. omega. Qed. 
+*)
+
+(*Lemma fold_equiv_blocks_SHA256 :
+  forall (l : Blist) (acc : Blist)
+         (L : list int) (ACC : list int),
+      InBlocks ShaInstantiation.b l ->
+      InBlocks 16 L ->
+      l = convert L ->
+      acc = convert ACC ->
+      hash_blocks_bits _ ShaInstantiation.B sha_h acc l = convert (hash_blocks ACC L).
+Proof. intros. eapply fold_equiv_blocks.
+  3: apply SHA256.hash_blocks_equation.
+  reflexivity. reflexivity. trivial. trivial. trivial. trivial.
+Qed.
+
+Lemma splitandpad_equiv : forall (bits : Blist) (bytes : list Z),
+                            bytes_bits_lists bits bytes ->
+                            bytes_bits_lists
+                              (sha_splitandpad bits)
+                              (pad bytes).
+Proof.
+  intros bits bytes inputs_eq.
+  unfold concat.
+  unfold sha_splitandpad.
+  specialize (bytesBitsLists_isbyteZ _ _ inputs_eq). intros isbyteZ_Bytes.
+
+  apply bytes_bits_ind_comp in inputs_eq. 2: apply isbyteZ_Bytes.
+  rewrite inputs_eq.
+  apply bytes_bits_def_eq.
+  rewrite <- inputs_eq. apply pad_isbyteZ. trivial.
+Qed.
+*)
+
+Lemma gap_divide16 bits: NPeano.divide 16 (length (generate_and_pad' (bitsToBytes bits))).
+Proof.
+    unfold generate_and_pad'.
+    destruct (pad_len_64_nat (bitsToBytes bits)).
+     rewrite pure_lemmas.length_Zlist_to_intlist with (n:=(x*16)%nat). 
+       exists x. trivial.
+     rewrite H. unfold WORD. rewrite (mult_comm (Z.to_nat 4)). rewrite mult_comm.
+        rewrite <- mult_assoc. reflexivity.
+Qed.
+
+Lemma equiv_pad_SHA256 : forall (bits : Blist) (bytes : list Z),
+                    bytes_bits_lists bits bytes ->
+                    bytes_bits_lists
+                      (HMAC_Pad.hash_words_padded c p B sha_h sha_iv sha_splitandpad bits)
+                      (HP.SHA256.Hash bytes).
+Proof. intros.
+  eapply HMAC_Pad.equiv_pad with (gap:=generate_and_pad').
+  2: reflexivity.
+  2: apply hash_blocks_equation.
+  reflexivity. reflexivity.
+  apply gap_divide16.
+  intros. unfold sha_splitandpad. f_equal. 
+    apply bytes_bits_ind_comp in H.
+    { subst bytes. unfold generate_and_pad'.
+      rewrite pure_lemmas.Zlist_to_intlist_to_Zlist; trivial.
+        destruct (pad_len_64_nat (bitsToBytes bits0)). rewrite H.
+          exists ((x*16)%nat). rewrite mult_comm, <- mult_assoc. reflexivity.
+        apply pad_isbyteZ. eapply bitsToBytes_isbyteZ. reflexivity. }
+    apply (bytesBitsLists_isbyteZ _ _ H).
+  intros; unfold HP.SHA256.Hash.
+    rewrite -> functional_prog.SHA_256'_eq. unfold SHA256.SHA_256.
+    rewrite <- pad_compose_equal; reflexivity.
+  assumption.
+Qed.
+
+(* Relates the HMAC padded spec to the HMAC functional program *)
+Theorem HMAC_pad_concrete (K : list byte) (M H : list Z) (OP IP : Z)
+                          (k m h : Blist) (op ip : Blist) (ipByte: isbyteZ IP) (opByte: isbyteZ OP):
+  ((length K) * 8)%nat = (c + p)%nat ->
+  Zlength K = Z.of_nat HP.SHA256.BlockSize ->
+  bytes_bits_lists k (map Byte.unsigned K) ->
+  bytes_bits_lists m M ->
+  bytes_bits_lists op (HP.HMAC_SHA256.sixtyfour OP) ->
+  bytes_bits_lists ip (HP.HMAC_SHA256.sixtyfour IP) ->
+  HMAC_Pad.HMAC c p B sha_h sha_iv sha_splitandpad op ip k m = h ->
+  HP.HMAC_SHA256.HmacCore (Byte.repr IP) (Byte.repr OP) M K = H ->
+  bytes_bits_lists h H.
+Proof.
+  intros padded_key_len padded_key_len_byte padded_keys_eq msgs_eq ops_eq ips_eq.
+  intros HMAC_abstract HMAC_concrete.
+
+  intros.
+
+  rewrite <- HMAC_abstract. rewrite <- HMAC_concrete.
+
+  unfold HMAC_Pad.HMAC. unfold HP.HMAC_SHA256.HmacCore. unfold HP.HMAC_SHA256.OUTER. unfold HP.HMAC_SHA256.INNER.
+  unfold HP.HMAC_SHA256.outerArg. unfold HP.HMAC_SHA256.innerArg.
+
+  unfold HMAC_Pad.HMAC_2K. unfold HMAC_Pad.GHMAC_2K. rewrite -> split_append_id.
+
+  { apply equiv_pad_SHA256.
+    apply bytes_bits_lists_append.
+    apply xor_equiv_byte; trivial. 
+
+    apply equiv_pad_SHA256.
+    apply bytes_bits_lists_append.
+    - apply xor_equiv_byte; trivial.
+    - assumption. }
+  { apply BLxor_length; erewrite bytes_bits_length; try eassumption.
+         rewrite map_length, padded_key_len. reflexivity.
+         unfold HP.HMAC_SHA256.sixtyfour.
+         rewrite -> length_list_repeat. reflexivity. }
+  { apply BLxor_length; erewrite bytes_bits_length; try eassumption.
+         rewrite map_length, padded_key_len. reflexivity.
+         unfold HP.HMAC_SHA256.sixtyfour.
+         rewrite -> length_list_repeat. reflexivity. }
+Qed.
+
+Theorem HMAC_pad_concrete' (K : list byte) (M : list Z) (OP IP : Z)
+                           (k m : Blist) (op ip : Blist) (ipByte: isbyteZ IP) (opByte: isbyteZ OP):
+  ((length K) * 8)%nat = (c + p)%nat ->
+  Zlength K = Z.of_nat HP.SHA256.BlockSize ->
+  bytes_bits_lists k (map Byte.unsigned K) ->
+  bytes_bits_lists m M ->
+  bytes_bits_lists op (HP.HMAC_SHA256.sixtyfour OP) ->
+  bytes_bits_lists ip (HP.HMAC_SHA256.sixtyfour IP) ->
+  HMAC_Pad.HMAC c p B sha_h sha_iv sha_splitandpad op ip k m = 
+  bytesToBits (HP.HMAC_SHA256.HmacCore (Byte.repr IP) (Byte.repr OP) M K).
+Proof. intros.  
+  eapply bits_bytes_ind_comp.
+    apply isbyte_hmaccore.
+    eapply (HMAC_pad_concrete _ ipByte opByte); try reflexivity; trivial. 
+Qed.
