sha/HMAC_isPRF.v
@@ -16,6 +16,9 @@ Require Import sha_padding_lemmas.
 Require Import SHA256.
 Require Import pure_lemmas.
 Require Import HMAC_equivalence.
+Require Import ShaInstantiation.
+Require Import HMAC256_spec_pad.
+Require Import HMAC256_spec_list.
 
 Lemma splitAndPad_v_to_sha_splitandpad_blocks l:
    map Vector.to_list (splitAndPad_v l) = sha_splitandpad_blocks l.
@@ -38,8 +41,8 @@ Proof. intros.
   apply bytesToBits_injective in B. 
     apply pad_inc_injective in B.
     apply (bitsToBytes_injective8 _ _ B L1 L2).
-  apply isbyteZ_pad_inc. eapply HMAC_spec_pad.HMAC_Pad.bitsToBytes_isbyteZ. reflexivity.
-  apply isbyteZ_pad_inc. eapply HMAC_spec_pad.HMAC_Pad.bitsToBytes_isbyteZ. reflexivity.
+  apply isbyteZ_pad_inc. eapply bitsToBytes_isbyteZ. reflexivity.
+  apply isbyteZ_pad_inc. eapply bitsToBytes_isbyteZ. reflexivity.
 Qed.
 
 Lemma opad_ne_ipad : opad_v <> ipad_v.
@@ -68,20 +71,20 @@ Definition isPRF {D R Key:Set} (RndKey:Comp Key) (RndR: Comp R) (f: Key -> D -> 
 Variable P : Blist -> Prop.
 Variable HP: forall m, P m -> NPeano.divide 8 (length m).
 
-Lemma wrappedSAP_1_1_local (msg1 msg2 : Message P):
-      wrappedSAP splitAndPad_v msg1 = wrappedSAP splitAndPad_v msg2 -> msg1 = msg2.
-Proof. apply wrappedSAP_1_1. intros.
+Lemma wrappedSAP_1_1_local (msg1 msg2 : HMAC_Abstract.Message P):
+      HMAC_Abstract.wrappedSAP _ _ splitAndPad_v msg1 = HMAC_Abstract.wrappedSAP _ _ splitAndPad_v msg2 -> msg1 = msg2.
+Proof. apply HMAC_Abstract.wrappedSAP_1_1. intros.
   apply HP in H0; apply HP in H1.
   apply splitAndPad_1to1; trivial.
 Qed. 
 
-Definition msg_eqb (msg1 msg2:Message P): bool.
+Definition msg_eqb (msg1 msg2:HMAC_Abstract.Message P): bool.
 destruct msg1 as [m1 M1].
 destruct msg2 as [m2 M2].
 apply (list_EqDec bool_EqDec). apply m1. apply m2.
 Defined.
 
-Lemma Message_eqdec: EqDec (Message P).
+Lemma Message_eqdec: EqDec (HMAC_Abstract.Message P).
 apply (Build_EqDec msg_eqb). 
 intros; unfold msg_eqb. destruct x as [m1 M1]. destruct y as [m2 M2].
 destruct (eqb_leibniz m1 m2). 
@@ -91,62 +94,35 @@ split; intros.
 Qed.
 
 (* Assume h is a tau-PRF against adversary (PRF_h_A h_star_pad A_GHMAC) *)
-Definition h_PRF (A : OracleComp (Message P) (Bvector c) bool) tau := 
+Definition h_PRF (A : OracleComp (HMAC_Abstract.Message P) (Bvector c) bool) tau := 
            isPRF ({ 0 , 1 }^c) ({ 0 , 1 }^c) h_v (Bvector_EqDec (b c p)) (Bvector_EqDec c) tau 
                          (PRF_h_A (h_star_pad h_v fpad_v) 
-                                  (HMAC_PRF.A_GHMAC p Message_eqdec (wrappedSAP splitAndPad_v) A)).
+                                  (HMAC_PRF.A_GHMAC p Message_eqdec (HMAC_Abstract.wrappedSAP _ _ splitAndPad_v) A)).
 
 (* We could make similar predicates for the other definitions, or just
 assume the inequalities*)
-Definition h_star_WCR (A : OracleComp (Message P) (Bvector c) bool) epsilon := 
+Definition h_star_WCR (A : OracleComp (HMAC_Abstract.Message P) (Bvector c) bool) epsilon := 
        cAU.Adv_WCR (list_EqDec (Bvector_EqDec (b c p)))
              (Bvector_EqDec (b c p)) (h_star_pad h_v fpad_v)
-       ({ 0 , 1 }^c) (au_F_A (A_GHMAC p Message_eqdec (wrappedSAP splitAndPad_v) A)) <= epsilon.
+       ({ 0 , 1 }^c) (au_F_A (A_GHMAC p Message_eqdec (HMAC_Abstract.wrappedSAP _ _ splitAndPad_v) A)) <= epsilon.
 
-Definition dual_h_RKA (A : OracleComp (Message P) (Bvector c) bool) sigma:=
+Definition dual_h_RKA (A : OracleComp (HMAC_Abstract.Message P) (Bvector c) bool) sigma:=
     RKA_Advantage _ _ _ ({ 0 , 1 }^b c p) ({ 0 , 1 }^c) (dual_f h_v) (BVxor (b c p))
-      (HMAC_RKA_A h_v iv_v fpad_v opad_v ipad_v (A_GHMAC p Message_eqdec (wrappedSAP splitAndPad_v) A)) <= sigma.
+      (HMAC_RKA_A h_v iv_v fpad_v opad_v ipad_v (A_GHMAC p Message_eqdec (HMAC_Abstract.wrappedSAP _ _ splitAndPad_v) A)) <= sigma.
 
 Theorem HMAC_isPRF A (A_wf : well_formed_oc A) tau epsilon sigma 
         (HH1: h_PRF A tau) (HH2: h_star_WCR A epsilon) (HH3: dual_h_RKA A sigma):
         isPRF (Rnd (b c p)) (Rnd c) 
-              (HMAC h_v iv_v (wrappedSAP splitAndPad_v)
+              (HMAC h_v iv_v (HMAC_Abstract.wrappedSAP _ _ splitAndPad_v)
                               fpad_v opad_v ipad_v)
               Message_eqdec _ (tau + epsilon + sigma) A.
 Proof. unfold isPRF.
-  specialize (HMAC_PRF h_v iv_v Message_eqdec (wrappedSAP splitAndPad_v) wrappedSAP_1_1_local
+  eapply leRat_trans. 
+    apply (HMAC_PRF h_v iv_v Message_eqdec (HMAC_Abstract.wrappedSAP _ _ splitAndPad_v) wrappedSAP_1_1_local
                               fpad_v opad_ne_ipad A_wf).
-  intros.
-  eapply leRat_trans. apply H. clear H. 
-  unfold h_PRF, isPRF in HH1.
-  unfold HMAC_common_defs.b in *. unfold HMAC_spec.b in *. unfold b in *. 
-    unfold GHMAC_PRF.b in *. unfold GNMAC_PRF.b in *.  unfold HMAC_spec.b in *.
-  remember (@PRF_Advantage (Bvector (c + p)) (Bvector c) (Bvector c) ({ 0 , 1 }^c)
-        ({ 0 , 1 }^c) h_v (Bvector_EqDec (c + p)) (Bvector_EqDec c)
-        (@PRF_h_A (c + p) c c (@h_star_pad c p h_v fpad_v)
-           (@A_GHMAC c p (Message P) Message_eqdec
-              (@wrappedSAP P splitAndPad_v) A))). clear Heqr.
-  unfold h_star_WCR in HH2.
-  unfold HMAC_common_defs.b in *. unfold HMAC_spec.b in *. unfold b in *.
-    unfold GHMAC_PRF.b in *. unfold GNMAC_PRF.b in *.  unfold HMAC_spec.b in *.
-  remember (@cAU.Adv_WCR (Bvector c) (list (Bvector (c + p))) (Bvector (c + p))
-        (@list_EqDec (Bvector (c + p)) (Bvector_EqDec (c + p)))
-        (Bvector_EqDec (c + p)) (@h_star_pad c p h_v fpad_v) ({ 0 , 1 }^c)
-        (@au_F_A (c + p) c
-           (@A_GHMAC c p (Message P) Message_eqdec
-              (@wrappedSAP P splitAndPad_v) A))). clear Heqr0.
-  unfold dual_h_RKA in HH3.
-  unfold HMAC_common_defs.b in *. unfold HMAC_spec.b in *. unfold b in *.
-    unfold GHMAC_PRF.b in *. unfold GNMAC_PRF.b in *.  unfold HMAC_spec.b in *.
-  remember (@RKA_Advantage (Bvector (c + p)) (Bvector c) (Bvector c)
-        (Bvector (c + p)) (Bvector_EqDec (c + p)) (Bvector_EqDec c)
-        (Bvector_EqDec c) ({ 0 , 1 }^c + p) ({ 0 , 1 }^c)
-        (@dual_f (Bvector c) (Bvector (c + p)) (Bvector c) h_v)
-        (BVxor (c + p))
-        (@HMAC_RKA_A c p h_v iv_v fpad_v opad_v ipad_v
-           (@A_GHMAC c p (Message P) Message_eqdec
-              (@wrappedSAP P splitAndPad_v) A))). clear Heqr1.
   rewrite ratAdd_comm. 
-  apply ratAdd_leRat_compat; trivial. apply ratAdd_leRat_compat; trivial. (*What's the "omega" tactic for Rat?*)
+  apply ratAdd_leRat_compat.
+    apply ratAdd_leRat_compat. apply HH1. apply HH2.
+    apply HH3.
 Qed.
 End HMAC_is_PRF. 
