sha/hmac_common_lemmas.v
@@ -3,10 +3,11 @@
 Require Import Integers.
 Require Import Coqlib.
 Require Import List. Import ListNotations.
-Require Import SHA256.
-Require Import sha.spec_sha.
-Require Import pure_lemmas.     (* sha *)
+Require Import general_lemmas.
 Require Import hmac_pure_lemmas.
+Require Import SHA256.
+Require Import pure_lemmas.     (* sha *)
+Require Import sha.spec_sha.
 
 Require Import HMAC_functional_prog.
 
@@ -14,78 +15,9 @@ Lemma SF_ByteRepr x: isbyteZ x ->
                      HP.HMAC_SHA256.sixtyfour x = 
                      map Byte.unsigned (HP.HMAC_SHA256.sixtyfour (Byte.repr x)).
 Proof. intros. unfold HP.HMAC_SHA256.sixtyfour.
- rewrite pure_lemmas.map_list_repeat.
+ rewrite map_list_repeat.
  rewrite Byte.unsigned_repr; trivial. destruct H. 
  assert (BMU: Byte.max_unsigned = 255). reflexivity. omega.
-Qed.
-
-Lemma NPeano_divide_trans a b c: NPeano.divide a b -> 
-      NPeano.divide b c -> NPeano.divide a c.
-Proof. intros. destruct H; destruct H0. subst.
-  exists (x0 * x)%nat. apply mult_assoc.
-Qed. 
-
-Lemma isByte_mono: forall x y, 0<=y<=x -> isbyteZ x -> isbyteZ y.
-Proof. intros. destruct H0. split; omega. Qed.
-
-Lemma length_mul_split A k (K:(0<k)%nat) n (N:(0<n)%nat): forall (l:list A), length l = (k * n)%nat -> 
-      exists l1, exists l2, l=l1++l2 /\ length l1=n /\ length l2 = ((k-1) * n)%nat.
-Proof.
-  intros. 
-  assert ((k * n = n + (k-1) * n)%nat). rewrite mult_minus_distr_r. simpl. rewrite plus_0_r.  
-      rewrite NPeano.Nat.add_sub_assoc. rewrite minus_plus. trivial.
-      specialize (mult_le_compat_r 1 k n). simpl; rewrite plus_0_r. simpl; intros. apply H0. omega.
-  rewrite H0 in H; clear H0. 
-  apply (list_splitLength _ _ _ H).
-Qed.   
-
-Lemma app_inv_length1 {A}: forall (l1 m1 l2 m2:list A),
-  l1++l2 = m1++m2 -> length l1 = length m1 -> l1=m1 /\ l2=m2.
-Proof.
-induction l1; simpl; intros.
-{ destruct m1; simpl in *. split; trivial. omega. }
-{ destruct m1; simpl in *. discriminate.
-  inversion H; clear H; subst a0.
-  destruct (IHl1 _ _ _ H3). omega.
-  subst. split; trivial. }
-Qed.
-
-Lemma app_inv_length2 {A}: forall (l1 m1 l2 m2:list A),
-  l1++l2 = m1++m2 -> length l2 = length m2 -> l1=m1 /\ l2=m2.
-Proof.
-induction l1; simpl; intros.
-{ destruct m1; simpl in *. split; trivial.
-  assert (length l2 = length (a :: m1 ++ m2)). rewrite <- H; trivial.
-  rewrite H1 in H0; clear H H1. simpl in H0. rewrite app_length in H0. omega. }
-{ assert (length (a :: l1 ++ l2) = length (m1 ++ m2)). rewrite <- H; trivial.
-  simpl in H1. do 2 rewrite app_length in H1. rewrite H0 in H1.
-  destruct m1; simpl in *. omega.
-  inversion H; clear H. subst a0.
-  destruct (IHl1 _ _ _ H4 H0). subst. split; trivial. }
-Qed.
-
-Lemma cons_inv {A}: forall (a1 a2:A) t1 t2, a1::t1 = a2::t2 -> a1=a2 /\ t1=t2.
-  intros. inversion H; split; trivial. Qed.
-
-Lemma mod_exists a b c: a mod b = c -> b<> 0 -> exists k, k*b+c=a.
-Proof. intros. specialize (Zmod_eq_full a b H0). intros.
-  exists (a/b). rewrite H in H1; clear H H0. subst c. omega. Qed.
-
-Lemma Forall2_map {A B} (f:A -> B): forall l m, 
-      Forall2 (fun x y => y = f x) l m -> map f l = m.
-Proof. intros.
-  induction H; simpl. reflexivity.
-  subst y. f_equal. trivial.
-Qed.
-
-Lemma app_inj1 {A} l2 m2: forall (l1 m1:list A) (H:l1++l2=m1++m2),
-      length l1=length m1 -> l1=m1 /\ l2=m2.
-Proof. induction l1.
-  destruct m1; simpl; intros. split; trivial. discriminate.
-  destruct m1; simpl; intros. discriminate.
-  inversion H; subst. 
-  destruct (IHl1 _ H3). omega.
-  subst. split; trivial.
 Qed.
 
 Lemma str_to_Z_length: forall k, 
@@ -115,30 +47,6 @@ Proof. unfold isbyteZ, HP.HMAC_SHA256.zeroPad; intros.
   apply in_app_or in H0.
   destruct H0. apply (H _ H0).
   apply in_list_repeat in H0. (*apply In_Nlist in H0.*) subst; omega.
-Qed.
-
-Lemma unsigned_Brepr_isbyte z: isbyteZ z -> Byte.unsigned (Byte.repr z) = z.
-Proof. intros. 
-      unfold isbyteZ in H. apply Byte.unsigned_repr.
-      unfold Byte.max_unsigned, Byte.modulus. simpl. omega.
-Qed.  
-
-Lemma map_unsigned_Brepr_isbyte: forall l, Forall isbyteZ l ->
-      map Byte.unsigned (map Byte.repr l) = l.
-Proof. intros. induction l; simpl in *. trivial.
-   rewrite IHl. rewrite Forall_forall in H. 
-   assert (In a (a::l)). left. trivial. 
-   specialize (H _ H0); clear H0.
-   rewrite unsigned_Brepr_isbyte; trivial.
-   rewrite Forall_forall in *. intros. apply H. right; trivial.
-Qed.
-
-Lemma isByte_ByteUnsigned b: isbyteZ (Byte.unsigned b).
-Proof.
-  unfold Byte.unsigned, Byte.intval. destruct b.
-  unfold Byte.modulus, Byte.wordsize, Wordsize_8.wordsize in intrange.
-  rewrite two_power_nat_correct in intrange.
-  unfold Zpower_nat in intrange. simpl in intrange. unfold isbyteZ. omega.
 Qed.
 
 Lemma nth_zeropad_left {d d'}: forall l i (I: 0<= i < Zlength l),
@@ -175,7 +83,6 @@ Proof. unfold HP.HMAC_SHA256.zeroPad.
     omega.
 Qed.
 
-
 Lemma mkKey_right {d}: forall l (L: false = (Zlength l >? 64)) 
         i (I: Zlength l <= i < 64),
       nth (Z.to_nat i) (HP.HMAC_SHA256.mkKey l) d = Z0.
@@ -183,15 +90,6 @@ Proof.
   unfold HP.HMAC_SHA256.mkKey. intros. simpl. rewrite <- L.
   apply nth_zeropad_right; trivial.
 Qed.
-
-Lemma isbyte_map_ByteUnsigned l: Forall isbyteZ (map Byte.unsigned l).
-Proof. 
-  rewrite Forall_forall. intros. 
-  apply list_in_map_inv in H. destruct H as [b [B1 _]]. subst x.
-  apply isByte_ByteUnsigned.
-Qed.
-
-(* HP.SHA256_ changed *)
 
 Lemma zeroPad_BlockSize: forall k, (length k <= HP.SHA256.BlockSize)%nat ->
   length (HP.HMAC_SHA256.zeroPad k) = HP.SHA256.BlockSize%nat.
@@ -203,7 +101,6 @@ Lemma length_SHA256': forall l,
 Proof. intros. unfold functional_prog.SHA_256'. simpl.
   rewrite length_intlist_to_Zlist, functional_prog.length_process_msg. reflexivity.
 Qed.
- 
 
 Lemma mkKey_length l: length (HP.HMAC_SHA256.mkKey l) = HP.SHA256.BlockSize.
 Proof. intros. unfold HP.HMAC_SHA256.mkKey.
@@ -224,22 +121,6 @@ Proof. unfold HP.HMAC_SHA256.mkKey. rewrite Zlength_correct.
   simpl. unfold HP.HMAC_SHA256.zeroPad. rewrite H. simpl.
   apply app_nil_r.  
 Qed.
-
-Lemma isbyteZ_xor a b: isbyteZ a -> isbyteZ b -> isbyteZ (Z.lxor a b).
-Proof. intros. rewrite xor_inrange.
-        apply Z_mod_lt. omega.
-        symmetry; apply Zmod_small. apply H.
-        symmetry; apply Zmod_small. apply H0.
-Qed.
-
-Lemma unsigned_repr_isbyte x:
-  isbyteZ x -> Int.unsigned (Int.repr x) = x.
-Proof. intros; apply Int.unsigned_repr. 
-  rewrite int_max_unsigned_eq. destruct H; omega. 
-Qed.
-
-Lemma isbyteZ_range q: isbyteZ q -> 0 <= q <= Byte.max_unsigned. 
-Proof. intros B; destruct B. unfold Byte.max_unsigned, Byte.modulus; simpl. omega. Qed.
 
 Lemma isbyte_sha x: Forall isbyteZ (functional_prog.SHA_256' x).
 Proof. apply isbyte_intlist_to_Zlist. Qed.
@@ -265,7 +146,7 @@ Proof. intros. inversion H; clear H.
   repeat rewrite <- Z.add_assoc.
   assert (Zlength blocks * WORD * 8 + Zlength newfrag * 8 =
           Zlength oldfrag * 8 + Zlength L * 8).
-    assert (Zlength (oldfrag ++ L) = Zlength (SHA256.intlist_to_Zlist blocks ++ newfrag)).
+    assert (Zlength (oldfrag ++ L) = Zlength (intlist_to_Zlist blocks ++ newfrag)).
       rewrite H4; trivial.
     clear H4. rewrite Zlength_app in H.
               rewrite <- (Z.mul_add_distr_r (Zlength oldfrag)), H. clear H.
